@@ -2,16 +2,17 @@ module
 
 public import Roolean.QfBv.Domain.Bitvector
 
-public class AbstractDomain (α : Type) [Domain α] where
-  top: Nat → α
-  containsConcrete: α → Bitvector → Bool
-  split: α → Nat → (α × Option α)
+public class AbstractDomain (α : Nat → Type) [Domain α] where
+  top (w: Nat) : α w
+  containsConcrete {w}: α w → Bitvector w → Bool
+  split {w}: α w → Nat → (α w × Option (α w))
 
-  top_containsConcrete_all : c.width = w → containsConcrete (top w) c
-  containsConcrete_nonempty : ∃x, containsConcrete a x
-  split_noop_id : split a n = (b, none) → a = b
-  split_preserves : split a n = (left, some right) →
-    containsConcrete a c → containsConcrete left c ∨ containsConcrete right c
+  top_containsConcrete_all {w} (c: Bitvector w) : containsConcrete (top w) c
+  containsConcrete_nonempty {w} (a: α w) : ∃c, containsConcrete a c
+  split_noop_id {w} (a b : α w) (n: Nat) : split a n = (b, none) → a = b
+  split_preserves {w} (a left right : α w) (n: Nat) (c: Bitvector w)
+    : split a n = (left, some right) → containsConcrete a c →
+      containsConcrete left c ∨ containsConcrete right c
 
-  uniOp_sound : Domain.uniOp a op = Except.ok ar → containsConcrete a c →
-    Bitvector.uniOp c op = Except.ok cr ∧ containsConcrete ar cr
+  uniOp_sound {w} (a ar: α w) (op: DomainUniOp) (c: Bitvector w)
+    : containsConcrete a c → containsConcrete (Domain.uniOp a op) (c.uniOp op)
